coq-osiris/theories/program_logic/fun_spec.v
@@ -472,3 +472,172 @@ Section ewp_EApp_def.
   Qed.
 
 End ewp_EApp_def.
+
+Section ewpi_EApp_prop_aux_def.
+
+  Context `{!osirisGS Σ}.
+  Context (ι : thread) (η : env) (Ψ : iEff Σ).
+  Context (expr_base : expr) (goal_prop : expr -> iProp Σ).
+
+  (* [accumulate_argument_premises_and_build_consequence_hyp] builds up
+     premises for each argument and a consequence hypothesis. *)
+
+  Equations iaccumulate_argument_premises_and_build_consequence_hyp
+    (τ : types) (es : list expr) (conseq_acc : τ -#> iProp Σ -> iProp Σ) :
+    iProp Σ :=
+  | Tbase X, es, conseq_acc :=
+      ∀ (e : expr) (φ : X -> iProp Σ),
+        EWP[ι] eval η e <|Ψ|> {{ ensures #x, φ x }} -∗
+        (* [Hconseq] is the consequence premise built over all parameters *)
+        let Hconseq := ∀ (x : X), conseq_acc x (φ x) in
+        (* [nested_eapp] is the nested application *)
+        let nested_eapp := app_exprs expr_base (e :: es) in
+        Hconseq -∗ goal_prop (nested_eapp)
+  | type_nel.Tcons X τ', es, conseq_acc :=
+      ∀ (e : expr) (φ : X -> iProp Σ),
+        EWP[ι] eval η e <|Ψ|> {{ ensures #x, φ x }} -∗
+        let conseq_acc :=
+          (λ# (tt : τ') (Q : iProp Σ),
+              ∀ (x : X),
+                φ x -∗
+                (tapp (conseq_acc x) tt) Q)
+        in
+        iaccumulate_argument_premises_and_build_consequence_hyp
+          τ' (e :: es) conseq_acc.
+
+  Arguments iaccumulate_argument_premises_and_build_consequence_hyp !τ /.
+  Transparent iaccumulate_argument_premises_and_build_consequence_hyp.
+  Strategy transparent [ iaccumulate_argument_premises_and_build_consequence_hyp ].
+
+  (* Monotonicity of the accumulator *)
+
+  Lemma ewpi_EApp_mono (τ : types) es (Hmon' Hmon : τ -#> iProp Σ -> iProp Σ) :
+    iaccumulate_argument_premises_and_build_consequence_hyp τ es Hmon' -∗
+    □ (∀ args (P : iProp Σ), Hmon args P -∗ Hmon' args P) -∗
+    iaccumulate_argument_premises_and_build_consequence_hyp τ es Hmon.
+  Proof.
+    revert es.
+    induction τ as [ X HX | X HX τ IH ]; iIntros (es) "HEApp' #Hmono"; simpl.
+    - iIntros (ex φx) "Hex Hx". cbn zeta.
+      iSpecialize ("HEApp'" $! ex φx with "Hex"). cbn zeta.
+      iApply "HEApp'".
+      iIntros (v). iApply ("Hmono" with "Hx").
+    - iIntros (ex φx) "Hex".
+      iApply (IH with "[HEApp' Hex]").
+      + iApply ("HEApp'" with "Hex").
+      + iModIntro. iIntros (args P). rewrite !tapp_bind.
+        iIntros "Hx" (x) "Hφx".
+        iApply ("Hmono" $! (x, args) P).
+        iApply ("Hx" with "Hφx").
+  Qed.
+
+End ewpi_EApp_prop_aux_def.
+
+Section ewpi_EApp_def.
+  Context `{!osirisGS Σ}.
+
+  Definition ewpi_EApp_prop `{Encode A} (τ : types) : iProp Σ :=
+    ∀ (ι : thread) (η : env) (e : expr) (Ψ' : A -> iProp Σ) (Ψ : iEff Σ)
+      (P : τ -#> microvx -> iProp Σ),
+    EWP[ι] eval η e <|Ψ|> {{ ensures c, iSpec τ c P }} -∗
+    iaccumulate_argument_premises_and_build_consequence_hyp
+      ι η Ψ e
+      (λ e, EWP[ι] eval η e <|Ψ|> {{ ensures #v, Ψ' v }})
+      τ
+      []
+      (λ# (tt : τ) (Q : iProp Σ),
+           Q -∗ ∀ m, (tapp P tt) m -∗ ▷ EWP[ι] m <|Ψ|> {{ ensures #v, Ψ' v }}).
+
+  Arguments ewpi_EApp_prop {_ _} !τ /.
+  Transparent ewpi_EApp_prop.
+  Strategy transparent [ ewpi_EApp_prop ].
+
+  (* Helper lemma for the induction step *)
+
+  Lemma ewpi_EApp_prop_induction_step
+    ι (τ : types) (η : env) (Ψ : iEff Σ) e (g : expr -> iProp Σ) :
+    ∀ (Hconseq : τ -#> iProp Σ -> iProp Σ) (es : list expr) (ei : expr),
+      app_exprs (EApp e ei) es = app_exprs e (es ++ [ei]) →
+      iaccumulate_argument_premises_and_build_consequence_hyp
+        ι η Ψ (EApp e ei) g τ es Hconseq -∗
+      iaccumulate_argument_premises_and_build_consequence_hyp
+        ι η Ψ e g τ (es ++ [ei]) Hconseq.
+  Proof.
+    induction τ as [ X HX | X HX τ IH ]; iIntros (Hconseq es ei HeqEApp) "Happlied".
+    - (* Base case *)
+      simpl in *. rewrite <- HeqEApp. iApply "Happlied".
+    - (* Inductive case *)
+      iIntros (ex φx) "Hex". cbn zeta.
+      iApply (IH (λ# (tt : τ) (B : iProp Σ),
+                   ∀ x : X,
+                     φx x -∗
+                     tapp Hconseq (x, tt) B)%I
+                 (ex :: es) ei).
+      + simpl. f_equal. apply HeqEApp.
+      + iApply ("Happlied" with "Hex").
+  Qed.
+
+  (* Main lemma for n-ary function application *)
+
+  Lemma ewpi_EApp `{Encode A} (τ : types) :
+    ⊢ @ewpi_EApp_prop A _ τ.
+  Proof.
+    induction τ as [ X HX | X HX τ IH].
+    - (* Base case *)
+      unfold ewp_EApp_prop.
+      iIntros (ι η e Ψ' Ψ P) "HSpec"; iIntros (ex φx) "Hex"; cbn zeta.
+      iIntros "Hmono".
+      simpl_eval.
+      iApply (ewpi_Par with "HSpec Hex").
+      + iIntros (?) "[]".
+      + iIntros (?) "[]".
+      + iIntros (c v) "HSpec' Hφx". simpl. simp iSpec.
+        iDestruct "Hφx" as (x) "[-> Hφx]".
+        iApply ("Hmono" with "Hφx HSpec'").
+
+    - (* Inductive case: multi-argument function *)
+      unfold ewpi_EApp_prop.
+      iIntros (ι η e Ψ' Ψ P) "HSpec"; iIntros (ex φx) "Hex".
+      change [ex] with ([] ++ [ex]).
+    iApply (ewpi_EApp_prop_induction_step ι τ η Ψ e
+              (λ e, EWP[ι] eval η e <|Ψ|> {{ ensures #x, Ψ' x }})%I); first reflexivity.
+
+    (* Define the intermediate specification P' *)
+    set (P' := (λ# (tt : τ) m,
+                 ∃ x : X,
+                   φx x ∗
+                   tapp P (x, tt) m)%I : τ -#> microvx -> iProp Σ).
+
+    (* Use IH *)
+    iPoseProof IH as "HIH".
+    unfold ewp_EApp_prop.
+    iSpecialize ("HIH" $! ι η (EApp e ex) _ _ P' with "[HSpec Hex]").
+    { simpl_eval.
+      iApply (ewpi_Par with "HSpec Hex").
+      - iIntros (? []).
+      - iIntros (? []).
+      -
+        iIntros (??) "HSpec (%x & -> & Hφx) /=".
+        simp iSpec.
+        iSpecialize ("HSpec" $! x ι).
+        iPoseProof (ewpi_prot_mono with "[] HSpec") as "HSpec"; last first.
+        iApply (ewpi_mono with "HSpec").
+        iIntros ([|]); [ | iIntros ([]) ].
+        iIntros "!> HSpec /=".
+        iApply (iSpec_mono with "HSpec").
+        rewrite bi_tforall_equiv.
+        iIntros (xs m) "HP".
+        subst P'. cbn. rewrite tapp_bind.
+        iFrame. iApply iEff_le_bottom. }
+
+    (* Apply monotonicity *)
+    iApply (ewpi_EApp_mono with "HIH").
+
+    iIntros "!>" (args Q). rewrite !tapp_bind.
+    iIntros "H HQ %m (%x & Hφx & HP)".
+    iSpecialize ("H" $! x with "Hφx").
+    rewrite tapp_bind.
+    iApply ("H" with "HQ HP").
+  Qed.
+
+End ewpi_EApp_def.
